Re-prove lemmas and VCs for a revolving door requirement

Barrier/Requirements.thy
@@ -12,10 +12,15 @@ definition R3 where "R3 s \<equiv> toEnvP s \<and>
 P6_2 s (\<lambda> s1. getVarBool s1 down' = True) (\<lambda> s2. getVarBool s2 closed' = True) (\<lambda> s3. getVarBool s3 up' = False)
  (\<lambda> s4. getVarBool s4 carInFront' = False) (\<lambda> s5. getVarBool s5 carInFront' = True)"
 
+definition R4Pattern where "R4Pattern s t A1 A2 A3 A4 A5 A6 A7 \<equiv> P1' s t A1 (\<lambda> s2. (previous_all s2 A2 \<or> A3 s2) \<and> A4 s2) (\<lambda> s3. (previous_ex s3 A5 \<and> A6 s3) \<or> A7 s3)"
+
+
 definition R4 where "R4 s \<equiv> toEnvP s \<and>
-(\<forall> s1. substate s1 s \<and> toEnvP s1 \<and> toEnvNum s1 s \<ge> OPEN_TIME'TIMEOUT \<and> getVarBool s1 green' = True \<longrightarrow>
-(\<exists> s3. toEnvP s3 \<and> substate s1 s3 \<and> substate s3 s \<and> toEnvNum s1 s3 \<le> OPEN_TIME'TIMEOUT \<and> (getVarBool s3 down' = True \<or> getVarBool s3 peCarUnder' = True ) \<and>
-(\<forall> s2. toEnvP s2 \<and> substate s1 s2 \<and> substate s2 s3 \<and> s2 \<noteq> s3 \<longrightarrow> getVarBool s2 down' = False \<and> getVarBool s2 peCarUnder' = False)))"
+R4Pattern s (OPEN_TIME'TIMEOUT - 1) (\<lambda> s1. getVarBool s1 green' = True) (\<lambda> s2. getVarBool s2 carInFront' = True) (\<lambda> s3. getVarBool s3 carInFront' = False)
+(\<lambda> s4. getVarBool s4 down' = False \<and> getVarBool s4 opened' = True \<and> getVarBool s4 peCarUnder' = False) 
+(\<lambda> s2. getVarBool s2 carInFront' = False) (\<lambda> s3. getVarBool s3 carInFront' = True)
+(\<lambda> s4. getVarBool s4 down' = True \<and> getVarBool s4 opened' = False \<and> getVarBool s4 peCarUnder' = True) "
+
 
 definition R5 where "R5 s \<equiv> toEnvP s \<and>
 (\<forall> s1 s2. substate s1 s2 \<and> substate s2 s \<and> toEnvP s1 \<and> toEnvP s2 \<and> toEnvNum s1 s2 = 1 \<and>
