Pattern2_Def.thy
@@ -11,6 +11,9 @@ definition previous_ex where "previous_ex s A \<equiv>
 definition always2 where  "always2 s A1 A2 A3 \<equiv> 
 always s (\<lambda> s2.( previous_ex s2 A1) \<and> A2 s2 \<longrightarrow> A3 s2)"
 
+definition always2_inv where  "always2_inv s b A1 A2 A3 \<equiv> 
+always s (\<lambda> s2.( previous_ex s2 A1) \<and> A2 s2 \<longrightarrow> A3 s2) \<and> (b \<longrightarrow> \<not>A1 s)"
+
 lemma previous_all_one_point: "consecutive s0 s \<Longrightarrow>  A s0 \<Longrightarrow> previous_all s A"
   apply(unfold  previous_all_def)
   apply simp
@@ -32,15 +35,48 @@ lemma previous_ex_rule: "
   apply(unfold previous_ex_def)
   by (meson consecutive.simps substate_trans)
 
-lemma always2_rule: "consecutive s0 s \<Longrightarrow>
-always2 s0 A1 A2 A3 \<and> (\<not> A1 s0 \<or> ~ A2 s \<or> A3' s) \<and> (\<forall> s1. toEnvP s1 \<and> substate s1 s0 \<and> A3 s1 \<longrightarrow> A3' s1) \<Longrightarrow> always2 s A1 A2 A3'"
-  apply(unfold always2_def)
-  by (smt (verit) always_def consecutive.elims(2) previous_ex_def substate_noteq_imp_substate_of_pred toEnvNum_eq_imp_eq2)
+lemma previous_ex_not: "\<not> previous_ex s A \<longleftrightarrow> previous_all s (\<lambda> s0. \<not> A s0)"
+  using previous_all_def previous_ex_def by presburger
 
+lemma always2_rule: "
+always2_inv s0 b A1 A2 A3 \<Longrightarrow>consecutive s0 s \<Longrightarrow> (((b \<or> ~ A2 s) \<or> A3' s) \<and> (\<forall> s1. toEnvP s1 \<and> substate s1 s0 \<and> A3 s1 \<longrightarrow> A3' s1)) \<and> (b' \<longrightarrow> \<not>A1 s) \<Longrightarrow>
+ always2_inv s b' A1 A2 A3'"
+  apply(unfold always2_inv_def)
+ (* by (smt (verit, ccfv_threshold) always_def consecutive.elims(2) previous_all_def previous_all_one_point previous_ex_def substate_noteq_imp_substate_of_pred)
+*)
+  apply(simp only: imp_conv_disj de_Morgan_conj previous_ex_not )
+  apply(erule conjE)
+  apply(erule conjE)
+  subgoal premises prems1
+    apply(rule conjI)
+     apply(insert prems1(1,2,4))[1]
+     apply(erule always_rule)
+      apply simp
+     apply(erule conjE)
+    subgoal premises prems2
+      apply(rule conjI)
+       apply(insert prems2(1,2))[1]
+       apply(erule disjE)
+        apply(rule disjI1)
+        apply(erule disjE)
+         apply(rule disjI1)
+         apply(rule previous_all_one_point[of s0])
+      apply simp
+      using prems1(3) apply simp
+        apply(rule disjI2)
+        apply assumption (*apply simp*)
+       apply(rule disjI2)
+       apply assumption
+      apply(insert prems2(1,3))[1]
+      apply auto
+      done
+    apply(insert prems1(1,3,5))
+    apply simp
+    done
+  done
 
-
-lemma always2_einv2req: "always2 s A1 A2 A3 \<and>  (\<forall> s1. toEnvP s1 \<and> substate s1 s \<and> A3 s1 \<longrightarrow> A3' s1) \<Longrightarrow> always2 s A1 A2 A3'"
-  apply(unfold always2_def)
-  by (simp add: always_def)
+lemma always2_einv2req: "always2_inv s b A1 A2 A3 \<Longrightarrow>  (\<forall> s1. toEnvP s1 \<and> substate s1 s \<and> A3 s1 \<longrightarrow> A3' s1) \<Longrightarrow> always2 s A1 A2 A3'"
+  apply(unfold always2_def always2_inv_def)
+  by (metis (mono_tags, lifting) always_einv2req)
 
 end
