Pattern4_Def.thy
@@ -1,5 +1,5 @@
 theory Pattern4_Def
-  imports VCTheoryLemmas
+  imports Pattern1_Def Pattern2_Def
 begin
 
 definition P4 where "P4 s t A1 A2 A3 \<equiv> 
@@ -14,43 +14,9 @@ definition P4inv where "P4inv s t t1 A1 A2 A3 \<equiv>
 toEnvNum s2 s < t1 \<and>
 (\<forall> s3. toEnvP s3 \<and> substate s2 s3 \<and> substate s3 s \<longrightarrow> A3 s3))"
 
-lemma P4inv_rule: "
-P1 \<longrightarrow> P4inv s0 t t1 A1 A2 A3 \<Longrightarrow> 
-P2 \<and> A1 s0 s \<longrightarrow> A2 s \<or> A3 s \<and> t2 > 0  \<Longrightarrow>
-P2 \<and> t1 > 0 \<longrightarrow> A2 s \<and> t1 \<le> t \<or> A3 s \<and> t1 < t2 \<Longrightarrow>
-P2 \<longrightarrow> P1 \<Longrightarrow> toEnvP s0 \<and> toEnvP s  \<and> substate s0 s \<and> toEnvNum s0 s = 1 \<Longrightarrow>
-P2 \<longrightarrow> P4inv s t t2 A1 A2 A3"
-  apply(rule impI)
-  apply simp
-  apply(rule cut_rl[of "\<forall> s1. substate s1 s \<and> toEnvP s1  \<and> s1 \<noteq> s \<longrightarrow> substate s1 s0"])
-   apply(unfold P4inv_def)[1]
-   apply(rule allI)+
-  subgoal for s1 s2
-    apply(cases "s2 = s")
-    apply (smt (verit, ccfv_threshold) bot_nat_0.extremum_uniqueI diff_add_0 diff_add_inverse2 less_add_eq_less linorder_le_cases plus_1_eq_Suc substate_antisym substate_toEnvNum_id substate_trans toEnvNum3 toEnvNum_id)
-      apply(rule impI)
-      apply(erule allE[of _ s1])
-    apply(rotate_tac -1)
-      apply(erule allE[of _ s2])
-    apply(rotate_tac -1)
-      apply(erule impE)
-     apply blast
-      apply(erule disjE)
-    using substate_trans apply blast
-     apply(rotate_tac 1)
-      apply(erule impE)
-       apply simp
-      apply(rotate_tac -1)
-      apply(erule disjE)
-       apply(rule disjI1)
-       apply(rule exI[of _ s])
-    apply (metis One_nat_def Suc_eq_plus1 Suc_leI dual_order.trans substate_refl toEnvNum3)
-    by (metis One_nat_def Suc_eq_plus1 less_trans_Suc toEnvNum3)
-  by (metis (full_types) add_is_1 substate_linear substate_toEnvNum_id toEnvNum3)
-
 lemma P4inv_rule2: "
  P4inv s0 t t1 A1 A2 A3 \<Longrightarrow> 
- A1 s0 s \<longrightarrow> A2 s \<or> A3 s \<and> t2 > 0  \<Longrightarrow>
+A1 s0 s \<longrightarrow> A2 s \<or> A3 s \<and> t2 > 0  \<Longrightarrow>
  t1 > 0 \<longrightarrow> A2 s \<and> t1 \<le> t \<or> A3 s \<and> t1 < t2 \<Longrightarrow>
  toEnvP s0 \<and> toEnvP s  \<and> substate s0 s \<and> toEnvNum s0 s = 1 \<Longrightarrow>
  P4inv s t t2 A1 A2 A3"
@@ -78,8 +44,8 @@ lemma P4inv_rule2: "
        apply(rule exI[of _ s])
     apply (metis One_nat_def Suc_eq_plus1 Suc_leI dual_order.trans substate_refl toEnvNum3)
     by (metis One_nat_def Suc_eq_plus1 less_trans_Suc toEnvNum3)
-  by (metis (full_types) add_is_1 nat_1 nat_one_as_int substate_linear substate_toEnvNum_id toEnvNum3)
-   
+  using substate_noteq_imp_substate_of_pred by blast
+
 lemma einv2req: "
 P4inv s t t1 A1 A2 A3 \<Longrightarrow> t1 \<le> t \<Longrightarrow>
 (\<forall> s1 s2. substate s1 s2 \<and> substate s2 s \<and> toEnvP s1 \<and> toEnvP s2 \<and> toEnvNum s1 s2 = 1\<and>  toEnvNum s2 s \<ge> t \<and> A1 s1 s2 \<longrightarrow>
@@ -93,5 +59,97 @@ P4inv s t t1 A1 A2 A3 \<Longrightarrow> t1 \<le> t \<Longrightarrow> P4 s t A1 A
   apply(unfold P4inv_def P4_def)
   by (smt (verit, best) leD le_eq_less_or_eq order_less_trans)
 
+definition P4' where "P4' s t A1 A2 A3 A4 \<equiv>
+always2 s A1 A2 (\<lambda> s2. constrained_until s2 s t A3 A4)"
+
+definition P4'inv where "P4'inv s t t1 b A1 A2 A3 A4 \<equiv>
+always2_inv s b A1 A2 (\<lambda> s2. constrained_until_inv s2 s t t1 A3 A4)"
+
+
+lemma P4'inv_rule: "
+ P4'inv s0 t t1 b A1 A2 A3 A4 \<Longrightarrow> 
+(((b \<or> \<not> A2 s) \<or> A4 s \<or> A3 s \<and> t2 > 0)  \<and>
+(t1 = 0 \<or> A4 s \<and> t1 \<le> t \<or> A3 s \<and> t1 < t2)) \<and> (b' \<longrightarrow> \<not> A1 s)  \<Longrightarrow>
+consecutive s0 s \<Longrightarrow>
+ P4'inv s t t2 b' A1 A2 A3 A4"
+  apply(unfold P4'inv_def)
+  apply(erule always2_rule)
+   apply simp
+  apply(erule conjE)
+  subgoal premises prems1
+    apply(rule conjI)
+     apply(insert prems1(1,2))[1]
+     apply(erule conjE)
+    subgoal premises prems2
+      apply(rule conjI)
+       apply(insert prems2(1,2))[1]
+       apply(erule disjE)
+        apply(rule disjI1)
+        apply assumption
+       apply(rule disjI2)
+       apply(rule constrained_until_one_point)
+        apply simp
+       apply assumption
+      apply(insert prems2(1,3))
+      apply(rule constrained_until_rule)
+       apply simp
+      apply(rule conjI)
+       apply(rule all_imp_refl)
+      apply(rule conjI)
+       apply simp
+      apply assumption
+      done
+    apply(insert prems1(1,3))
+    apply simp
+    done
+  done
+
+lemma P4'inv_rule_gen: "
+ P4'inv s0 t t1 b A1 A2 A3 A4 \<Longrightarrow> consecutive s0 s \<Longrightarrow>
+(((b \<or> \<not> A2 s) \<or> A4' s \<or> A3' s \<and> t2 > 0)  \<and>
+( \<forall>s1. toEnvP s1 \<and> substate s1 s0 \<and> A3 s1 \<longrightarrow> A3' s1) \<and>
+( \<forall>s1. toEnvP s1 \<and> substate s1 s0 \<and> A4 s1 \<longrightarrow> A4' s1) \<and>
+(t1 = 0 \<or> A4' s \<and> t1 \<le> t \<or> A3' s \<and> t1 < t2)) \<and> (b' \<longrightarrow> \<not> A1 s)  \<Longrightarrow>
+
+ P4'inv s t t2 b' A1 A2 A3' A4'"
+  apply(unfold P4'inv_def)
+  apply(erule always2_rule)
+   apply simp
+  apply(erule conjE)
+  subgoal premises prems1
+    apply(rule conjI)
+     apply(insert prems1(1,2))[1]
+     apply(erule conjE)
+    subgoal premises prems2
+      apply(rule conjI)
+       apply(insert prems2(1,2))[1]
+       apply(erule disjE)
+        apply(rule disjI1)
+        apply assumption
+       apply(rule disjI2)
+       apply(rule constrained_until_one_point)
+        apply simp
+       apply assumption
+      apply(insert prems2(1,3))
+      apply(rule constrained_until_rule)
+       apply simp
+      apply assumption
+      done
+    apply(insert prems1(1,3))
+    apply simp
+    done
+  done
+
+lemma P4'_einv2req_gen: "P4'inv s t t1 b A1 A2 A3 A4 \<Longrightarrow>(\<forall> s1. toEnvP s1 \<and> substate s1 s \<and> A3 s1 \<longrightarrow> A3' s1) \<and> (\<forall> s1. toEnvP s1 \<and> substate s1 s \<and> A4 s1 \<longrightarrow> A4' s1) \<and>
+ t1 \<le> t \<Longrightarrow> P4' s t A1 A2 A3' A4'"
+  apply(unfold P4'_def P4'inv_def)
+  using always2_einv2req constrained_until_einv2req
+  by simp
+
+
+lemma P4'_einv2req: "P4'inv s t t1 b A1 A2 A3 A4 \<Longrightarrow> t1 \<le> t \<Longrightarrow> P4' s t A1 A2 A3 A4"
+  apply(unfold P4'_def P4'inv_def)
+  using always2_einv2req constrained_until_einv2req
+  by (smt (verit, best))
+
 end
-  
