Pattern3_Def.thy
@@ -5,8 +5,8 @@ begin
 definition always where "always s A \<equiv>
 \<forall> s1. substate s1 s \<and> toEnvP s1 \<longrightarrow> A s1"
 
-lemma always_rule: "always s0 A \<and> (A' s) \<and> (\<forall> s1 . toEnvP s1 \<and> substate s1 s0 \<and>A s1 \<longrightarrow> A' s1) \<Longrightarrow>
-consecutive s0 s \<Longrightarrow> always s A'"
+lemma always_rule: "always s0 A \<Longrightarrow>consecutive s0 s \<Longrightarrow> (A' s) \<and> (\<forall> s1 . toEnvP s1 \<and> substate s1 s0 \<and>A s1 \<longrightarrow> A' s1) \<Longrightarrow>
+ always s A'"
   apply(unfold always_def)
   by (metis consecutive.elims(2) substate_noteq_imp_substate_of_pred)
 
