Patterns.thy
@@ -6,6 +6,7 @@ Pattern4_Def
 Pattern5_Def
 Pattern6_Def
 Pattern7_Def
+Pattern9_def
 Pattern10_Def
 Pattern11_Def
 Pattern12_Def
