RequirementLemmas.thy
@@ -7,7 +7,12 @@ lemma all_disj_rule: "(\<forall> s1. toEnvP s1 \<and> substate s1 s \<and> P s1 
   apply auto
   done
 
-lemma all_imp_refl: "True \<Longrightarrow> \<forall> s1. toEnvP s1 \<and> substate s1 s \<and> P s1 \<longrightarrow> P s1"
+lemma all_conj_rule: "(\<forall> s1. toEnvP s1 \<and> substate s1 s \<and> P s1 \<longrightarrow> P' s1) \<and> (\<forall> s1. toEnvP s1 \<and> substate s1 s \<and> Q s1 \<longrightarrow> Q' s1) \<Longrightarrow>
+\<forall> s1. toEnvP s1 \<and> substate s1 s \<and> (P s1 \<and> Q s1) \<longrightarrow> (P' s1 \<and> Q' s1)"
+  apply auto
+  done
+
+lemma all_imp_refl: " \<forall> s1. toEnvP s1 \<and> substate s1 s \<and> P s1 \<longrightarrow> P s1"
   apply auto
   done 
 
