RevolvingDoor/ExtraInv4_VC11.thy
@@ -1,0 +1,9 @@
+theory ExtraInv4_VC11
+  imports ExtraInv4
+begin
+
+theorem "VC11 extraInv env s0 user_value pressure_value"
+  apply(unfold VC11_def)
+  by simp
+
+end
