RevolvingDoor/ExtraInv4_VC13.thy
@@ -1,0 +1,30 @@
+theory ExtraInv4_VC13
+  imports ExtraInv4
+begin
+
+theorem "VC13 extraInv env s0 user_value pressure_value"
+  apply(unfold VC13_def extraInv_def)
+  apply(rule impI)
+  apply(rule conjI)
+  apply simp
+  apply(erule conjE)
+  subgoal premises vc_prems
+    apply(insert vc_prems(1))
+    apply(erule conjE)+
+    subgoal premises ei
+      apply(insert vc_prems(2)[simplified] ei(2))
+      apply rule
+       apply((rule P9inv_simp[OF ei(5)]);auto)
+      apply rule
+       apply simp
+      apply rule
+       apply simp
+      apply rule
+      using ei(6) apply simp
+      apply rule
+      using ei(7) apply simp
+      using ei(8) by simp
+    done
+  done
+
+end
