RevolvingDoor/Proof_R4_VC2.thy
@@ -1,0 +1,25 @@
+theory Proof_R4_VC2
+  imports ExtraInv4_VC2
+begin
+
+definition inv4 where "inv4 s \<equiv> extraInv s \<and> R4_1 s"
+
+theorem "VC2 inv4 env s0 user_value pressure_value"
+  apply(unfold VC2_def inv4_def R4_1_def)
+  apply rule
+  apply(rule context_conjI)
+  using extra2 apply(auto simp add: VC2_def)[1]
+  apply rule
+   apply simp
+  apply(erule conjE)
+  subgoal premises prems
+        apply(insert prems(1))
+    apply(unfold extraInv_def)
+    apply(erule conjE)+
+    subgoal premises ei
+      apply(rule einv2req)
+      using ei(3) prems(3)[simplified] by auto
+    done
+  done
+
+end
